Better concat rule; use define.

markov/bin2unary.lisp
@@ -5,242 +5,299 @@
 
 (defconst *scheme-bin2unary-en*
   (list
-    (mks->  "|0" "0||")
-    (mks->  "1"  "0|" )
-    (mks->  "0"  ""   )))
+    (mk-> '(! 0) '(0 ! !))
+    (mk-> '(1)   '(0 !))
+    (mk-> '(0)   '())))
 
 (defconst *scheme-bin2unary-ru*
   (list
-    (mks->  "1"  "0|" )
-    (mks->  "|0" "0||")
-    (mks->  "0"  ""   )))
+    (mk-> '(1)   '(0 !))
+    (mk-> '(! 0) '(0 ! !))
+    (mk-> '(0)   '())))
 
-(defund replace-ones (x)
-  (declare (xargs :guard t))
+(define replace-ones
+  ((x (wordp x '(0 1))))
+  :returns (result (wordp result '(0 !)) :hyp :guard)
   (cond ((atom x) nil)
-        ((eql (car x) #\1) (list* #\0 #\| (replace-ones (cdr x))))
-        (t (list* (car x) (replace-ones (cdr x))))))
+        ((eql (car x) '1) (list* '0 '! (replace-ones (cdr x))))
+        (t (list* (car x) (replace-ones (cdr x)))))
+  ///
+  (defrule |wordp-of-replace-ones|
+    (implies (and (wordp x '(0 1))
+                  (true-listp alphabet)
+                  (subsetp '(0 !) alphabet))
+             (wordp (replace-ones x) alphabet)))
+  (defrule |replace-ones append|
+    (equal (replace-ones (append x y))
+           (append (replace-ones x) (replace-ones y)))
+    :induct (len x)))
 
-(defruled |wordp replace-ones 0bar|
-  (implies (wordp x '(#\0 #\1))
-           (wordp (replace-ones x) '(#\0 #\|)))
-  :enable replace-ones
-  :induct (len x))
+(define digit-count
+  ((x (wordp x '(0 1))))
+  :returns (result natp :rule-classes :type-prescription)
+  (cond ((atom x) 0)
+        ((or (eql (car x) '0) (eql (car x) '1)) (1+ (digit-count (cdr x))))
+        (t (digit-count (cdr x))))
+  ///
+  (defrule |digit-count append|
+    (equal (digit-count (append x y))
+           (+ (digit-count x) (digit-count y)))))
 
-(defrule |replace-ones append|
-  (equal (replace-ones (append x y))
-         (append (replace-ones x) (replace-ones y)))
-  :enable replace-ones
-  :induct (len x))
+(define val
+  ((x (wordp x '(0 1))))
+  :returns (val natp :rule-classes :type-prescription)
+  (cond ((atom x) 0)
+        ((or (eql (car x) '1) (eql (car x) '!))
+         (+ (expt 2 (digit-count (cdr x)))
+            (val (cdr x))))
+        (t (val (cdr x))))
+  ///
+  (defrule |val append|
+    (equal (val (append x y))
+           (+ (val y) (* (val x) (expt 2 (digit-count y)))))
+    :enable (digit-count append))
+  (defrule |duplicity bar <= val|
+    (<= (duplicity '! x)
+        (val x))
+    :enable duplicity
+    :rule-classes :linear)
+  (defrule |duplicity 1 <= val|
+    (<= (duplicity '1 x)
+        (val x))
+    :enable duplicity
+    :rule-classes :linear))
 
-(defund step1 (inp n)
-  (declare (xargs :guard (and (wordp inp'(#\0 #\1)) (natp n))))
-  (append (replace-ones (take n inp)) (nthcdr n inp)))
+;-------
 
-(defrule |step1 0|
-  (equal (step1 inp 0) inp)
-  :enable step1)
+(define step1
+  ((inp (wordp inp '(0 1)))
+   (n (and (natp n) (<= n (len inp)))))
+  :returns (result (wordp result '(0 1 !)) :hyp :guard)
+  (append (replace-ones (take n inp)) (nthcdr n inp))
+  ///
+  (defruled |step1 0|
+    (equal (step1 inp 0) inp))
+  (defruled |step1 len|
+    (implies
+     (wordp inp '(0 1))
+     (equal (step1 inp (len inp))
+            (replace-ones inp)))))
 
-(defrule |step1 len|
+(define step2
+  ((inp (wordp inp '(0 1)))
+   (n (and (natp n) (<= n (len inp)))))
+  :returns (result (wordp result '(0 !)) :hyp :guard)
+  (append (repeat n '0)
+          (repeat (val (take n inp)) '!)
+          (replace-ones (nthcdr n inp)))
+  ///
+  (defruled |step2 0|
+    (implies
+     (wordp inp '(0 1))
+     (equal (step2 inp 0)
+            (replace-ones inp))))
+  (defruled |step2 len|
+    (implies
+     (wordp inp '(0 1))
+     (equal (step2 inp (len inp))
+            (append (repeat (len inp) '0)
+                    (repeat (val inp) '!))))))
+
+(define step3
+  ((inp (wordp inp '(0 1)))
+   (n (and (natp n) (<= n (len inp)))))
+  :returns (result (wordp result '(0 !)))
+  (append (repeat (- (len inp) n) '0)
+          (repeat (val inp) '!))
+  ///
+  (defruled |step3 0|
+    (implies
+     (wordp inp '(0 1))
+     (equal (step3 inp 0)
+            (append (repeat (len inp) '0)
+                    (repeat (val inp) '!)))))
+  (defruled |step3 len|
+    (implies
+     (wordp inp '(0 1))
+     (equal (step3 inp (len inp))
+            (repeat (val inp) '!)))))
+
+(defruled |step2-0 as step1-len|
   (implies
-    (wordp inp'(#\0 #\1))
-    (equal (step1 inp (len inp))
-           (replace-ones inp)))
-  :enable step1)
+    (wordp inp '(0 1))
+    (equal (step2 inp 0)
+           (step1 inp (len inp))))
+  :enable (|step2 0| |step1 len|))
 
-(defrule |step1 same when #\0|
+(defruled |step3-0 as step2-len|
+  (implies
+    (wordp inp '(0 1))
+    (equal (step3 inp 0)
+           (step2 inp (len inp))))
+  :enable (|step3 0| |step2 len|))
+
+;------
+
+(define cnt
+  ((inp (wordp inp '(0 1))))
+  :returns (result natp :rule-classes :type-prescription)
+  (+ (val inp) (len inp)))
+
+(define step1-cntb
+  ((inp (wordp inp '(0 1)))
+   (n (and (natp n) (<= n (len inp)))))
+  (declare (ignore inp))
+  :returns (result natp :rule-classes :type-prescription
+                   :hyp (natp n))
+  n)
+
+(define step1-cntf
+  ((inp (wordp inp '(0 1)))
+   (n (and (natp n) (<= n (len inp)))))
+  :returns (result natp :rule-classes :type-prescription
+                   :hyp (and (natp n) (<= n (len inp))))
+  (+ (val inp) (len inp) (- n)))
+
+(defrule |step1 same when 0|
   (implies
     (and
-      (wordp inp'(#\0 #\1))
+      (wordp inp '(0 1))
       (natp n)
       (< n (len inp))
-      (eql (nth n inp) #\0))
+      (eql (nth n inp) '0))
     (equal (step1 inp (1+ n))
            (step1 inp n)))
   :enable (step1 |take n+1| |nthcdr as cons|))
 
-(defruled |step1 applicable when #\1|
+(defruled |step1 applicable when 1|
   (implies
     (and
-      (wordp inp'(#\0 #\1))
+      (wordp inp '(0 1))
       (natp n)
       (< n (len inp))
-      (eql (nth n inp) #\1))
+      (eql (nth n inp) '1))
    (equal
       (applicable *scheme-bin2unary-ru* (step1 inp n))
-      (mks-> "1" "0|")))
-  :enable (applicable step1 |wordp replace-ones 0bar|)
+      (mk-> '(1) '(0 !))))
+  :enable (applicable step1)
   :use (:instance sublistp-append-wordp
-         (pat '(#\1))
+         (pat '(1))
          (x (replace-ones (take n inp)))
-         (alphabet '(#\0 #\|))
+         (alphabet '(0 !))
          (y (nthcdr n inp))))
 
-(defruled |step1 substp when #\1|
+(defruled |step1 substp when 1|
   (implies
     (and
-      (wordp inp '(#\0 #\1))
+      (wordp inp '(0 1))
       (natp n)
       (< n (len inp))
-      (eql (nth n inp) #\1))
-    (substp (step1 inp n) '(#\1) '(#\0 #\|) (step1 inp (1+ n))))
+      (eql (nth n inp) '1))
+    (substp (step1 inp n) '(1) '(0 !) (step1 inp (1+ n))))
   :prep-lemmas (
     (defrule lemma
       (implies
-        (wordp x '(#\0 #\|))
-        (left-wingp x '(#\1)))
+        (wordp x '(0 !))
+        (left-wingp x '(1)))
       :enable (|left-wingp as left-wingp1| left-wingp1)
       :induct (len x)))
-  :enable (step1 |wordp replace-ones 0bar|
-           |take n+1| |nthcdr as cons|)
+  :enable (step1 |take n+1| |nthcdr as cons|)
   :use (:instance substp-lemma
          (x (step1 inp n))
-         (l '(#\1))
-         (r '(#\0 #\|))
+         (l '(1))
+         (r '(0 !))
          (y (step1 inp (1+ n)))
          (lw (replace-ones (take n inp)))
          (rw (nthcdr (1+ n) inp))))
 
-(defruled |step1 correct when #\1|
+(defruled |step1 correct when 1|
   (implies
     (and
-      (wordp inp '(#\0 #\1))
+      (wordp inp '(0 1))
       (natp n)
       (< n (len inp))
-      (eql (nth n inp) #\1))
+      (eql (nth n inp) '1))
     (simple-stepp
       *scheme-bin2unary-ru*
       (step1 inp n)
       (step1 inp (1+ n))))
-  :enable (simple-stepp |step1 applicable when #\1| |step1 substp when #\1|))
+  :enable (simple-stepp |step1 applicable when 1| |step1 substp when 1|))
 
 (defruled |step1 correct a|
   (implies
     (and
-      (wordp inp '(#\0 #\1))
+      (wordp inp '(0 1))
       (natp n)
       (< n (len inp)))
     (simple-steps
       *scheme-bin2unary-ru*
-      (if (eql (nth n inp) #\1) 1 0)
+      (if (eql (nth n inp) '1) 1 0)
       (step1 inp n)
       (step1 inp (1+ n))))
-  :enable |step1 correct when #\1|
+  :enable |step1 correct when 1|
   :disable |nth wordp is member|
   :use (:instance |nth wordp is member|
-         (alphabet '(#\0 #\1))
+         (alphabet '(0 1))
          (x inp)
          (i n)))
 
 (defruled |step1 correct all|
   (implies
     (and
-      (wordp inp '(#\0 #\1))
+      (wordp inp '(0 1))
       (natp n)
       (<= n (len inp)))
     (simple-steps
       *scheme-bin2unary-ru*
-      (duplicity #\1 (take n inp))
+      (duplicity '1 (take n inp))
       inp
       (step1 inp n)))
+  :enable |step1 0|
   :disable duplicity-of-append
   :induct (dec-induct n)
-  :hints (("subgoal *1/2" :do-not-induct t
-                          :use ((:instance simple-steps-cat
-                                  (scheme *scheme-bin2unary-ru*)
-                                  (m (duplicity #\1 (take (1- n) inp)))
-                                  (n (duplicity #\1 (list (nth (1- n) inp))))
-                                  (x inp)
-                                  (y (step1 inp (1- n)))
-                                  (z (step1 inp n)))
-                                (:instance |step1 correct a|
+  :hints (("subgoal *1/2" :use ((:instance |step1 correct a|
                                   (n (1- n)))
                                 (:instance duplicity-of-append
-                                  (a #\1)
+                                  (a '1)
                                   (x (take (1- n) inp))
                                   (y (list (nth (1- n) inp))))
                                 (:instance |take n+1|
                                   (x inp)
                                   (n (1- n)))))))
 
-(defund digit-count (x)
-  (declare (xargs :guard t))
-  (cond ((atom x) 0)
-        ((or (eql (car x) #\0) (eql (car x) #\1)) (1+ (digit-count (cdr x))))
-        (t (digit-count (cdr x)))))
-
-(defrule |digit-count append|
-  (equal (digit-count (append x y))
-         (+ (digit-count x) (digit-count y)))
-  :enable digit-count)
-
-(defund val (x)
-  (declare (xargs :guard t))
-  (cond ((atom x) 0)
-        ((or (eql (car x) #\1) (eql (car x) #\|))
-         (+ (expt 2 (digit-count (cdr x)))
-            (val (cdr x))))
-        (t (val (cdr x)))))
-
-(defrule |val append|
-  (equal (val (append x y))
-         (+ (val y) (* (val x) (expt 2 (digit-count y)))))
-  :prep-books ((include-book "arithmetic/top" :dir :system))
-  :enable (val digit-count append))
-
-(defrule |duplicity bar <= val|
-  (<= (duplicity #\| x)
-      (val x))
-  :prep-books ((include-book "arithmetic/top" :dir :system))
-  :enable (duplicity val)
-  :rule-classes :linear)
-
-(defrule |duplicity 1 <= val|
-  (<= (duplicity #\1 x)
-      (val x))
-  :prep-books ((include-book "arithmetic/top" :dir :system))
-  :enable (duplicity val)
-  :rule-classes :linear)
-
-(defund step2 (inp n)
-  (declare (xargs :guard (and (wordp inp '(#\0 #\1)) (natp n))))
-  (append (repeat n #\0)
-          (repeat (val (take n inp)) #\|)
-          (replace-ones (nthcdr n inp))))
-
 (defruled |step2 applicable|
   (implies
     (and
       (natp n)
       (posp i)
-      (wordp y '(#\0 #\|)))
+      (wordp y '(0 !)))
     (equal
       (applicable
         *scheme-bin2unary-ru*
-        (append (repeat n #\0) (repeat i #\|) (cons #\0 y)))
-      (mks-> "|0" "0||")))
+        (append (repeat n '0) (repeat i '!) (cons '0 y)))
+      (mk-> '(! 0) '(0 ! !))))
   :prep-lemmas (
     (defrule lemma1
       (implies
         (and (natp n)
              (posp i)
-             (wordp y '(#\0 #\|)))
-        (not (sublistp '(#\1)
-                       (append (repeat n #\0)
-                               (repeat i #\|)
-                               (cons #\0 y)))))
-      :cases ((sublistp '(#\1) y))
+             (wordp y '(0 !)))
+        (not (sublistp '(1)
+                       (append (repeat n '0)
+                               (repeat i '!)
+                               (cons '0 y)))))
+      :cases ((sublistp '(1) y))
       :hints (("subgoal 1" :use (:instance sublistp-append-wordp
-                                  (alphabet '(#\0 #\|))
-                                  (pat '(#\1))
+                                  (alphabet '(0 !))
+                                  (pat '(1))
                                   (x y)
                                   (y nil)))))
     (defrule lemma2
       (implies
          (posp i)
          (sublistp
-           '(#\| #\0)
-           (append (repeat i #\|) (cons #\0 y))))
+           '(! 0)
+           (append (repeat i '!) (cons '0 y))))
       :enable (sublistp repeat)
       :induct (dec-induct i)))
   :enable applicable)
@@ -252,26 +309,26 @@
       (posp i)
       (natp j))
     (substp
-      (append (repeat n #\0) (repeat i #\|) (list #\0) (repeat j #\|) y)
-      '(#\| #\0)
-      '(#\0 #\| #\|)
-      (append (repeat n #\0) (repeat (1- i) #\|) (list #\0) (repeat (+ 2 j) #\|) y)))
+      (append (repeat n '0) (repeat i '!) (list '0) (repeat j '!) y)
+      '(! 0)
+      '(0 ! !)
+      (append (repeat n '0) (repeat (1- i) '!) (list '0) (repeat (+ 2 j) '!) y)))
   :prep-lemmas (
     (defrule lemma1
       (implies (natp k)
-               (left-wingp1 (repeat k #\|) '(#\| #\0)))
+               (left-wingp1 (repeat k '!) '(! 0)))
       :enable (|left-wingp as left-wingp1| left-wingp1)
       :induct (dec-induct k)
-      :hints (("subgoal *1/2" :expand (repeat k #\|))))
+      :hints (("subgoal *1/2" :expand (repeat k '!))))
     (defrule lemma2
       (implies
         (and
           (natp n)
           (natp k))
-        (left-wingp (append (repeat n #\0) (repeat k #\|)) '(#\| #\0)))
+        (left-wingp (append (repeat n '0) (repeat k '!)) '(! 0)))
       :enable (|left-wingp as left-wingp1| left-wingp1)
       :induct (dec-induct n)
-      :hints (("subgoal *1/2" :expand (repeat n #\0))))
+      :hints (("subgoal *1/2" :expand (repeat n '0))))
     (defrule lemma3
       (implies
         (natp n)
@@ -285,12 +342,12 @@
        (equal (nthcdr n (append x y)) y))
      :induct (cdr-dec-induct x n)))
   :use (:instance substp-lemma
-         (x (append (repeat n #\0) (repeat i #\|) (list #\0) (repeat j #\|) y))
-         (l '(#\| #\0))
-         (r '(#\0 #\| #\|))
-         (y (append (repeat n #\0) (repeat (1- i) #\|) (list #\0) (repeat (+ 2 j) #\|) y))
-         (lw (append (repeat n #\0) (repeat (1- i) #\|)))
-         (rw (append (repeat j #\|) y))))
+         (x (append (repeat n '0) (repeat i '!) (list '0) (repeat j '!) y))
+         (l '(! 0))
+         (r '(0 ! !))
+         (y (append (repeat n '0) (repeat (1- i) '!) (list '0) (repeat (+ 2 j) '!) y))
+         (lw (append (repeat n '0) (repeat (1- i) '!)))
+         (rw (append (repeat j '!) y))))
 
 (defruled |step2 correct low|
   (implies
@@ -298,14 +355,14 @@
       (natp n)
       (posp i)
       (natp j)
-      (wordp y '(#\0 #\|)))
+      (wordp y '(0 !)))
     (simple-stepp
       *scheme-bin2unary-ru*
-      (append (repeat n #\0) (repeat i #\|) (list #\0) (repeat j #\|) y)
-      (append (repeat n #\0) (repeat (1- i) #\|) (list #\0) (repeat (+ 2 j) #\|) y)))
+      (append (repeat n '0) (repeat i '!) (list '0) (repeat j '!) y)
+      (append (repeat n '0) (repeat (1- i) '!) (list '0) (repeat (+ 2 j) '!) y)))
   :enable (simple-stepp wordp-repeat2)
   :use ((:instance |step2 applicable|
-          (y (append (repeat j #\|) y)))
+          (y (append (repeat j '!) y)))
         |step2 substp|))
 
 (defruled |step2 correct a|
@@ -314,12 +371,12 @@
       (natp n)
       (natp i)
       (natp j)
-      (wordp y '(#\0 #\|)))
+      (wordp y '(0 !)))
     (simple-steps
       *scheme-bin2unary-ru*
       i
-      (append (repeat n #\0) (repeat i #\|) (list #\0) (repeat j #\|) y)
-      (append (repeat n #\0) (list #\0) (repeat (+ (* 2 i) j) #\|) y)))
+      (append (repeat n '0) (repeat i '!) (list '0) (repeat j '!) y)
+      (append (repeat n '0) (list '0) (repeat (+ (* 2 i) j) '!) y)))
   :prep-lemmas (
     (defrule lemma1
       (implies
@@ -327,17 +384,17 @@
           (natp n)
           (posp i)
           (natp j)
-          (wordp y '(#\0 #\|)))
+          (wordp y '(0 !)))
         (simple-steps
           *scheme-bin2unary-ru*
           1
-          (append (repeat n #\0) (repeat i #\|) (list #\0) (repeat j #\|) y)
-          (append (repeat n #\0) (repeat (1- i) #\|) (list #\0) (repeat (+ 2 j) #\|) y)))
+          (append (repeat n '0) (repeat i '!) (list '0) (repeat j '!) y)
+          (append (repeat n '0) (repeat (1- i) '!) (list '0) (repeat (+ 2 j) '!) y)))
       :disable simple-steps-1
       :use ((:instance simple-steps-1
               (scheme *scheme-bin2unary-ru*)
-              (x (append (repeat n #\0) (repeat i #\|) (list #\0) (repeat j #\|) y))
-              (y (append (repeat n #\0) (repeat (1- i) #\|) (list #\0) (repeat (+ 2 j) #\|) y)))
+              (x (append (repeat n '0) (repeat i '!) (list '0) (repeat j '!) y))
+              (y (append (repeat n '0) (repeat (1- i) '!) (list '0) (repeat (+ 2 j) '!) y)))
             (:instance |step2 correct low|)))
     (defrule lemma
       (implies
@@ -346,49 +403,42 @@
           (natp i)
           (natp s)
           (<= (* 2 i) s)
-          (wordp y '(#\0 #\|)))
+          (wordp y '(0 !)))
         (simple-steps
           *scheme-bin2unary-ru*
           i
-          (append (repeat n #\0) (repeat i #\|) (list #\0) (repeat (- s (* 2 i)) #\|) y)
-          (append (repeat n #\0) (list #\0) (repeat s #\|) y)))
+          (append (repeat n '0) (repeat i '!) (list '0) (repeat (- s (* 2 i)) '!) y)
+          (append (repeat n '0) (list '0) (repeat s '!) y)))
     :induct (dec-induct i)
     :hints (
       ("subgoal *1/2" :use ((:instance lemma1
-                              (j (- s (* 2 i))))
-                            (:instance simple-steps-cat
-                              (scheme *scheme-bin2unary-ru*)
-                              (m 1)
-                              (n (1- i))
-                              (x (append (repeat n #\0) (repeat i #\|) (list #\0) (repeat (- s (* 2 i)) #\|) y))
-                              (y (append (repeat n #\0) (repeat (1- i) #\|) (list #\0) (repeat (- s (* 2 (1- i))) #\|) y))
-                              (z (append (repeat n #\0) (list #\0) (repeat s  #\|) y))))))))
+                              (j (- s (* 2 i)))))))))
   :use (:instance lemma
          (s (+ (* 2 i) j))))
 
 (defrule |val take n+1 inp|
   (implies
     (and
-      (wordp inp '(#\0 #\1))
+      (wordp inp '(0 1))
       (natp n)
       (< n (len inp)))
     (equal (val (take (+ 1 n) inp))
            (+ (* 2 (val (take n inp)))
-              (if (eql (nth n inp) #\1) 1 0))))
+              (if (eql (nth n inp) 1) 1 0))))
   :enable (|take n+1| digit-count)
   :disable |nth wordp is member|
   :use ((:instance |val append|
           (x (take n inp))
           (y (list (nth n inp))))
         (:instance |nth wordp is member|
-          (alphabet '(#\0 #\1))
+          (alphabet '(0 1))
           (x inp)
           (i n))))
 
 (defruled |step2 correct q|
   (implies
     (and
-      (wordp inp '(#\0 #\1))
+      (wordp inp '(0 1))
       (natp n)
       (< n (len inp)))
     (simple-steps
@@ -407,164 +457,131 @@
      (defrule lemma2
        (implies
          (and
-           (wordp inp '(#\0 #\1))
+           (wordp inp '(0 1))
            (natp n)
            (< n (len inp))
-           (not (equal (nth n inp) #\1)))
-         (equal (cons #\0 (replace-ones (nthcdr (+ 1 n) inp)))
+           (not (equal (nth n inp) 1)))
+         (equal (cons 0 (replace-ones (nthcdr (+ 1 n) inp)))
                 (replace-ones (nthcdr n inp))))
       :enable (|nthcdr as cons| replace-ones))
      (defrule lemma3
        (implies
          (and
-           (wordp inp '(#\0 #\1))
+           (wordp inp '(0 1))
            (natp n)
            (< n (len inp))
-           (equal (nth n inp) #\1))
-         (equal (list* #\0 #\| (replace-ones (nthcdr (+ 1 n) inp)))
+           (equal (nth n inp) 1))
+         (equal (list* '0 '! (replace-ones (nthcdr (+ 1 n) inp)))
                 (replace-ones (nthcdr n inp))))
       :enable (|nthcdr as cons| replace-ones)))
-  :enable (step2 |wordp replace-ones 0bar|)
+  :enable step2
   :use (:instance |step2 correct a|
          (i (val (take n inp)))
-         (j (if (eql (nth n inp) #\1) 1 0))
+         (j (if (eql (nth n inp) 1) 1 0))
          (y (replace-ones (nthcdr (1+ n) inp)))))
+
+(define step2-count
+  ((inp (wordp inp '(0 1)))
+   (n (and (natp n) (<= n (len inp)))))
+  :returns (result natp :rule-classes :type-prescription)
+  (- (val (take n inp))
+     (duplicity '1 (take n inp)))
+  ///
+  (defrule step2-count-0
+    (equal (step2-count inp 0) 0))
+  (defruled step2-count-diff
+    (implies (and (wordp inp '(0 1))
+                  (posp n)
+                  (<= n (len inp)))
+             (equal (- (step2-count inp n)
+                       (step2-count inp (1- n)))
+                    (val (take (1- n) inp))))
+    :use ((:instance duplicity-of-append
+            (a '1)
+            (x (take (+ -1 n) inp))
+            (y (list (nth n inp))))
+          (:instance |val take n+1 inp|
+            (n (1- n)))
+          (:instance |take n+1|
+            (x inp)
+            (n (1- n))))))
 
 (defruled |step2 correct 4|
   (implies
-    (and
-      (wordp inp '(#\0 #\1))
-      (natp n)
-      (<= n (len inp)))
-    (simple-steps
-      *scheme-bin2unary-ru*
-      (- (val (take n inp))
-         (duplicity #\1 (take n inp)))
+   (and
+    (wordp inp '(0 1))
+    (natp n)
+    (<= n (len inp)))
+   (simple-steps
+    *scheme-bin2unary-ru*
+    (step2-count inp n)
       (step2 inp 0)
       (step2 inp n)))
-  :prep-lemmas (
-    (defrule lemma
-      (implies
-        (and
-          (wordp inp '(#\0 #\1))
-          (posp n)
-          (<= n (len inp)))
-        (equal
-          (+ (val (take (+ -1 n) inp))
-             (val (take (+ -1 n) inp))
-             (- (duplicity #\1 (take (+ -1 n) inp))))
-          (+ (val (take n inp))
-             (- (duplicity #\1 (take n inp))))))
-      :use ((:instance duplicity-of-append
-              (a #\1)
-              (x (take (+ -1 n) inp))
-              (y (list (nth n inp))))
-            (:instance |val take n+1 inp|
-              (n (1- n)))
-            (:instance |take n+1|
-              (x inp)
-             (n (1- n))))))
+  :enable step2-count-diff
   :induct (dec-induct n)
-  :hints (
-    ("subgoal *1/2" :use ((:instance |step2 correct q|
-                            (n (1- n)))
-                          (:instance simple-steps-cat
-                              (scheme *scheme-bin2unary-ru*)
-                              (m (- (val (take (1- n) inp))
-                                    (duplicity #\1 (take (1- n) inp))))
-                              (n (val (take (1- n) inp)))
-                              (x (step2 inp 0))
-                              (y (step2 inp (1- n)))
-                              (z (step2 inp n)))))))
+  :hints (("subgoal *1/2" :use ((:instance |step2 correct q|
+                                  (n (1- n)))))))
 
 #|
-(step2 '(#\1 #\0 #\1) 0)
-(step2 '(#\1 #\0 #\1) 1)
-(step2 '(#\1 #\0 #\1) 2)
-(step2 '(#\1 #\0 #\1) 3)
+(step2 '(1 0 1) 0)
+(step2 '(1 0 1) 1)
+(step2 '(1 0 1) 2)
+(step2 '(1 0 1) 3)
 |#
-(defruled |step2 0|
-  (implies
-    (wordp inp '(#\0 #\1))
-    (equal (step2 inp 0)
-           (step1 inp (len inp))))
-  :enable step2)
-
-(defruled |step2 len|
-  (implies
-    (wordp inp '(#\0 #\1))
-    (equal (step2 inp (len inp))
-           (append (repeat (len inp) #\0)
-                   (repeat (val inp) #\|))))
-  :enable step2)
-
 (defruled |step1 and step2 correct|
   (implies
-    (wordp inp '(#\0 #\1))
+    (wordp inp '(0 1))
     (simple-steps
       *scheme-bin2unary-ru*
       (val inp)
       inp
-      (append (repeat (len inp) #\0)
-              (repeat (val inp) #\|))))
-  :enable (|step2 0| |step2 len|)
-  :use ((:instance simple-steps-cat
-         (scheme *scheme-bin2unary-ru*)
-         (m (duplicity #\1 inp))
-         (n (- (val inp) (duplicity #\1 inp)))
-         (x inp)
-         (y (step2 inp 0))
-         (z (append (repeat (len inp) #\0)
-                    (repeat (val inp) #\|))))
-        (:instance |step1 correct all|
+      (append (repeat (len inp) '0)
+              (repeat (val inp) '!))))
+  :enable (|step2-0 as step1-len| |step2 len| step2-count)
+  :use ((:instance |step1 correct all|
           (n (len inp)))
         (:instance |step2 correct 4|
           (n (len inp)))))
 
-(defund step3 (inp n)
-  (declare (xargs :guard (and (integerp n) (<= n (len inp)))))
-  (append (repeat (- (len inp) n) #\0)
-          (repeat (val inp) #\|)))
-
 (defruled |step3 applicable|
   (implies
     (and
-      (wordp inp '(#\0 #\1))
+      (wordp inp '(0 1))
       (natp n)
       (< n (len inp)))
    (equal
       (applicable *scheme-bin2unary-ru* (step3 inp n))
-      (mks-> "0" "")))
+      (mk-> '(0) '())))
   :prep-lemmas (
     (defrule lemma1
-      (not (sublistp '(#\1) (repeat n #\|)))
+      (not (sublistp '(1) (repeat n '!)))
       :enable (sublistp repeat)
       :induct (dec-induct n))
     (defrule lemma2
-      (not (equal #\0 (car (repeat n #\|))))
+      (not (equal '0 (car (repeat n '!))))
       :enable repeat)
     (defrule lemma3
       (implies
         (natp n)
-        (not (sublistp '(#\| #\0) (repeat n #\|))))
+        (not (sublistp '(! 0) (repeat n '!))))
       :enable (sublistp repeat prefixp)
       :induct (dec-induct n))
     (defrule lemma4
       (implies
         (posp n)
-        (sublistp '(#\0) (append (repeat n #\0) x)))
-      :expand (repeat n #\0)))
+        (sublistp '(0) (append (repeat n '0) x)))
+      :expand (repeat n '0)))
   :enable (applicable step3))
 
 (defruled |step3 substp|
   (implies
     (and
-      (wordp inp '(#\0 #\1))
+      (wordp inp '(0 1))
       (natp n)
       (< n (len inp)))
     (substp
       (step3 inp n)
-      '(#\0)
+      '(0)
       '()
       (step3 inp (1+ n))))
   :prep-lemmas (
@@ -574,7 +591,7 @@
   :enable (step3 repeat)
   :use (:instance substp-lemma
          (x (step3 inp n))
-         (l '(#\0))
+         (l '(0))
          (r '())
          (y (step3 inp (1+ n)))
          (lw '())
@@ -583,19 +600,21 @@
 (defruled |step3 correct a|
   (implies
     (and
-      (wordp inp '(#\0 #\1))
-      (natp n)
-      (< n (len inp)))
+      (wordp inp '(0 1))
+      (posp n)
+      (<= n (len inp)))
     (simple-stepp
       *scheme-bin2unary-ru*
-      (step3 inp n)
-      (step3 inp (1+ n))))
-  :enable (simple-stepp |step3 applicable| |step3 substp|))
+      (step3 inp (1- n))
+      (step3 inp n)))
+  :enable (simple-stepp |step3 applicable|)
+  :use (:instance |step3 substp|
+         (n (1- n))))
 
 (defruled |step3 correct b|
   (implies
     (and
-      (wordp inp '(#\0 #\1))
+      (wordp inp '(0 1))
       (natp n)
       (<= n (len inp)))
     (simple-steps
@@ -603,52 +622,23 @@
       n
       (step3 inp 0)
       (step3 inp n)))
-  :induct (dec-induct n)
-  :hints (("subgoal *1/2" :use ((:instance simple-steps-cat
-                                  (scheme *scheme-bin2unary-ru*)
-                                  (m (1- n))
-                                  (n 1)
-                                  (x (step3 inp 0))
-                                  (y (step3 inp (1- n)))
-                                  (z (step3 inp n)))
-                                (:instance |step3 correct a|
-                                  (n (1- n)))))))
-
-(defruled |step3 0|
-  (implies
-    (wordp inp '(#\0 #\1))
-    (equal (step3 inp 0)
-           (step2 inp (len inp))))
-  :enable (step3 |step2 len|))
-
-(defruled |step3 len|
-  (implies
-    (wordp inp '(#\0 #\1))
-    (equal (step3 inp (len inp))
-           (repeat (val inp) #\|)))
-  :enable step3)
+  :enable |step3 correct a|
+  :induct (dec-induct n))
 
 (defruled |step123 correct|
   (implies
-    (wordp inp '(#\0 #\1))
+    (wordp inp '(0 1))
     (simple-steps
-      *scheme-bin2unary-ru*
-      (+ (val inp) (len inp))
-      inp
-      (repeat (val inp) #\|)))
-  :enable (|step2 len| |step3 0| |step3 len|)
-  :use ((:instance simple-steps-cat
-          (scheme *scheme-bin2unary-ru*)
-          (m (val inp))
-          (n (len inp))
-          (x inp)
-          (y (step3 inp 0))
-          (z (step3 inp (len inp))))
-        |step1 and step2 correct|
+     *scheme-bin2unary-ru*
+     (cnt inp)
+     inp
+     (repeat (val inp) '!)))
+  :enable (|step2 len| |step3 0| |step3 len| cnt)
+  :use (|step1 and step2 correct|
         (:instance |step3 correct b|
           (n (len inp)))))
 
 (defruled |applicable final|
-  (not (applicable *scheme-bin2unary-ru* (repeat n #\|)))
+  (not (applicable *scheme-bin2unary-ru* (repeat n '!)))
   :enable (applicable repeat)
   :induct (dec-induct n))
